src/lowparse/LowParse.Low.VLData.fst
@@ -1,6 +1,6 @@
 module LowParse.Low.VLData
 include LowParse.Spec.VLData
-include LowParse.Low.Combinators
+include LowParse.Low.FLData
 
 module B = LowStar.Buffer
 module E = LowParse.BigEndianImpl.Low
@@ -58,9 +58,82 @@ let parse32_bounded_integer
   | 3 -> parse32_bounded_integer_3
   | 4 -> parse32_bounded_integer_4
 
-module U32 = FStar.UInt32
+module I32 = FStar.Int32
 
-(*
+inline_for_extraction
+let validate32_bounded_integer
+  (i: integer_size)
+  (i32: I32.t { I32.v i32 == i } )
+: Tot (validator32 (parse_bounded_integer i))
+= validate32_total_constant_size (parse_bounded_integer i) i32 ()
+
+module U32 = FStar.UInt32
+module Cast = FStar.Int.Cast
+
+inline_for_extraction
+let validate32_vldata_payload
+  (sz: integer_size)
+  (f: ((x: bounded_integer sz) -> GTot bool))
+  (f_lemma: ((x: bounded_integer sz) -> Lemma (f x == true ==> U32.v x < 2147483648)))
+  (#k: parser_kind)
+  (#t: Type0)
+  (#p: parser k t)
+  (v: validator32 p)
+  (i: bounded_integer sz { f i == true } )
+: Tot (validator32 (parse_vldata_payload sz f p i))
+= (* eta expansion needed because of `weaken` *)
+  fun input len ->
+    Classical.forall_intro f_lemma;
+    validate32_fldata v (U32.v i) (Cast.uint32_to_int32 i) input len
+
+inline_for_extraction
+let validate32_vldata_gen
+  (sz: integer_size)
+  (sz32: I32.t { I32.v sz32 == sz } )
+  (f: ((x: bounded_integer sz) -> GTot bool))
+  (f_lemma: ((x: bounded_integer sz) -> Lemma (f x == true ==> U32.v x < 2147483648)))
+  (f' : ((x: bounded_integer sz) -> Tot (y: bool { y == f x })))
+  (#k: parser_kind)
+  (#t: Type0)
+  (#p: parser k t)
+  (v32: validator32 p)
+: Tot (validator32 (parse_vldata_gen sz f p))
+= parse_fldata_and_then_cases_injective sz f p;
+  parse_vldata_gen_kind_correct sz;
+  validate32_filter_and_then
+    (validate32_bounded_integer sz sz32)
+    (parse32_bounded_integer sz)
+    f
+    f'
+    #_ #_ #(parse_vldata_payload sz f p)
+    (validate32_vldata_payload sz f f_lemma v32)
+    ()
+
+#set-options "--z3rlimit 32"
+
+inline_for_extraction
+let validate32_bounded_vldata
+  (min: nat)
+  (min32: U32.t)
+  (max: nat)
+  (max32: U32.t)
+  (#k: parser_kind)
+  (#t: Type0)
+  (#p: parser k t)
+  (v: validator32 p)
+  (sz32: I32.t)
+  (u: unit {
+    U32.v min32 == min /\
+    U32.v max32 == max /\
+    min <= max /\ max > 0 /\ max < 2147483648 /\
+    I32.v sz32 == log256' max
+  })
+: Tot (validator32 (parse_bounded_vldata min max p))
+= [@inline_let]
+  let sz : integer_size = log256' max in
+  fun input len ->
+    validate32_vldata_gen sz sz32 (in_bounds min max) (fun _ -> ()) (fun i -> not (U32.lt i min32 || U32.lt max32 i)) v input len
+
 inline_for_extraction
 let validate32_bounded_vldata_strong
   (min: nat)
@@ -76,18 +149,44 @@ let validate32_bounded_vldata_strong
   (u: unit {
     U32.v min32 == min /\
     U32.v max32 == max /\
-    min <= max /\ max > 0 /\ max < 4294967296 /\
+    min <= max /\ max > 0 /\ max < 2147483648 /\
     I32.v sz32 == log256' max
   })
 : Tot (validator32 (parse_bounded_vldata_strong min max s))
+= fun input len ->
+  validate32_bounded_vldata min min32 max max32 v sz32 () input len
+
+let accessor_bounded_vldata_payload
+  (min: nat)
+  (max: nat)
+  (#k: parser_kind)
+  (#t: Type0)
+  (p: parser k t)
+  (sz32: U32.t)
+  (u: unit {
+    min <= max /\ max > 0 /\ max < 4294967296 /\
+    U32.v sz32 == log256' max
+  })
+: Tot (accessor (parse_bounded_vldata min max p) p (fun x y -> y == x))
 = [@inline_let]
-  let _ = parse_bounded_vldata_correct min max p in
-  [@inline_let]
-  let sz : integer_size = (log256' max) in
-  fun input len ->
-  let res1 = validate32_total_constant_size (parse_bounded_integer sz) sz' () in
-  if res1 `I32.lt` 0l
-  then res1
-  else
-    let v1 = parse32_bounded_integer sz input in
-    
+  let sz = log256' max in
+  fun input ->
+  let h = HST.get () in
+  parse_bounded_vldata_elim_forall min max p (B.as_seq h input);
+  let len = parse32_bounded_integer sz input in
+  B.sub (B.offset input sz32) 0ul len
+
+let accessor_bounded_vldata_strong_payload
+  (min: nat)
+  (max: nat)
+  (#k: parser_kind)
+  (#t: Type0)
+  (#p: parser k t)
+  (s: serializer p)
+  (sz32: U32.t)
+  (u: unit {
+    min <= max /\ max > 0 /\ max < 4294967296 /\
+    U32.v sz32 == log256' max
+  })
+: Tot (accessor (parse_bounded_vldata_strong min max s) p (fun x y -> y == x))
+= fun input -> accessor_bounded_vldata_payload min max p sz32 () input
