src/lowparse/LowParse.Low.fst
@@ -5,4 +5,5 @@ include LowParse.Low.Int
 include LowParse.Low.List
 include LowParse.Low.FLData
 include LowParse.Low.Array
-include LowParse.Bytes
+include LowParse.Low.Bytes
+include LowParse.Low.VLData
